playing with total mst

experiments/dm4ms/TOTAL_MST.fst
@@ -6,116 +6,116 @@ open WMonad
 open FStar.Tactics
 module W = FStar.Monotonic.Witnessed
 
-noeq type mheap = {
+noeq type tstate = {
   t: Type0;
   rel: FStar.Preorder.preorder t;
 }
 
-let stable (#heap) (pred:heap.t -> Type0) =
-  forall h1 h2. (pred h1 /\ h1 `heap.rel` h2) ==> pred h2
+let stable (#state) (pred:state.t -> Type0) =
+  forall h1 h2. (pred h1 /\ h1 `state.rel` h2) ==> pred h2
 
 noeq
-type free (heap:mheap) (a:Type u#a) : Type u#(max 1 a) =
-| Get : cont:(heap.t -> free heap a) -> free heap a
-| Put : heap.t -> cont:(unit -> free heap a) -> free heap a
-| Witness : p:(heap.t -> Type0) -> cont:(unit -> free heap a) -> free heap a
-| Recall : p:(heap.t -> Type0) -> cont:(unit -> free heap a) -> free heap a
+type free (state:tstate) (a:Type u#a) : Type u#(max 1 a) =
+| Get : cont:(state.t -> free state a) -> free state a
+| Put : state.t -> cont:(unit -> free state a) -> free state a
+| Witness : p:(state.t -> Type0) -> cont:(unit -> free state a) -> free state a
+| Recall : p:(state.t -> Type0) -> cont:(unit -> free state a) -> free state a
 
-| PartialCall : (pre:pure_pre) -> cont:((squash pre) -> free u#a heap a) -> free heap a
-| Return : a -> free heap a
+| PartialCall : (pre:pure_pre) -> cont:((squash pre) -> free u#a state a) -> free state a
+| Return : a -> free state a
 
-let free_return (heap:mheap) (a:Type) (x:a) : free heap a =
+let free_return (state:tstate) (a:Type) (x:a) : free state a =
   Return x
 
 let rec free_bind
-  (heap:mheap)
+  (state:tstate)
   (a:Type u#a)
   (b:Type u#b)
-  (l : free heap a)
-  (k : a -> free heap b) :
-  free heap b =
+  (l : free state a)
+  (k : a -> free state b) :
+  free state b =
   match l with
   | Return x -> k x
-  | Get cont -> Get (fun x -> free_bind heap a b (cont x) k)
-  | Put h cont -> Put h (fun _ -> free_bind heap a b (cont ()) k)
-  | Witness pred cont -> Witness pred (fun _ -> free_bind heap a b (cont ()) k)
-  | Recall pred cont -> Recall pred (fun _ -> free_bind heap a b (cont ()) k)
+  | Get cont -> Get (fun x -> free_bind state a b (cont x) k)
+  | Put h cont -> Put h (fun _ -> free_bind state a b (cont ()) k)
+  | Witness pred cont -> Witness pred (fun _ -> free_bind state a b (cont ()) k)
+  | Recall pred cont -> Recall pred (fun _ -> free_bind state a b (cont ()) k)
   | PartialCall pre fnc ->
       PartialCall pre (fun _ ->
-        free_bind heap a b (fnc ()) k)
+        free_bind state a b (fnc ()) k)
 
-let partial_call_wp (heap:Type0) (pre:pure_pre) : st_wp_h heap (squash pre) = 
+let partial_call_wp (state:Type0) (pre:pure_pre) : st_wp_h state (squash pre) = 
   fun p h0 -> pre /\ p () h0
 
-val theta : #a:Type u#a -> #heap:mheap -> free heap a -> st_wp_h heap.t a
-let rec theta #a #heap m =
+val theta : #a:Type u#a -> #state:tstate -> free state a -> st_wp_h state.t a
+let rec theta #a #state m =
   match m with
-  | Return x -> st_return heap.t _ x
+  | Return x -> st_return state.t _ x
   | PartialCall pre k ->
-      st_bind_wp heap.t _ _ (partial_call_wp heap.t pre) (fun r -> theta (k r))
+      st_bind_wp state.t _ _ (partial_call_wp state.t pre) (fun r -> theta (k r))
   | Get k ->
-      st_bind_wp heap.t _ _ (fun p h -> p h h) (fun r -> theta (k r))
+      st_bind_wp state.t _ _ (fun p h -> p h h) (fun r -> theta (k r))
   | Put h1 k ->
-      st_bind_wp heap.t _ _ (fun p h0 -> h0 `heap.rel` h1 /\ p () h1) (fun r -> theta (k r))
+      st_bind_wp state.t _ _ (fun p h0 -> h0 `state.rel` h1 /\ p () h1) (fun r -> theta (k r))
   | Witness pred k ->
-      st_bind_wp heap.t _ _ (fun p h -> pred h /\ stable pred /\ (W.witnessed heap.rel pred ==> p () h)) (fun r -> theta (k r))
+      st_bind_wp state.t _ _ (fun p h -> pred h /\ stable pred /\ (W.witnessed state.rel pred ==> p () h)) (fun r -> theta (k r))
   | Recall pred k ->
-      st_bind_wp heap.t _ _ (fun p h -> W.witnessed heap.rel pred /\ (pred h ==> p () h)) (fun r -> theta (k r))
+      st_bind_wp state.t _ _ (fun p h -> W.witnessed state.rel pred /\ (pred h ==> p () h)) (fun r -> theta (k r))
 
-let mst (heap:mheap) (a:Type) (wp:st_wp_h heap.t a)=
-  m:(free heap a){theta m ⊑ wp}
+let mst (state:tstate) (a:Type) (wp:st_wp_h state.t a)=
+  m:(free state a){theta m ⊑ wp}
 
-let mst_return heap (a:Type) (x:a) : mst heap a (st_return heap.t _ x) =
-  free_return heap a x
+let mst_return state (a:Type) (x:a) : mst state a (st_return state.t _ x) =
+  free_return state a x
 
 let mst_bind
-  (#heap:mheap)
+  (#state:tstate)
   (#a : Type u#a)
   (#b : Type u#b)
-  (#wp_v : st_wp_h heap.t a)
-  (#wp_f: a -> st_wp_h heap.t b)
-  (v : mst heap a wp_v)
-  (f : (x:a -> mst heap b (wp_f x))) :
-  Tot (mst heap b (st_bind_wp heap.t a b wp_v wp_f)) =
+  (#wp_v : st_wp_h state.t a)
+  (#wp_f: a -> st_wp_h state.t b)
+  (v : mst state a wp_v)
+  (f : (x:a -> mst state b (wp_f x))) :
+  Tot (mst state b (st_bind_wp state.t a b wp_v wp_f)) =
   admit (); (* TODO: prove monad morphism *)
-  free_bind heap a b v f
+  free_bind state a b v f
 
 let mst_subcomp
-  (#heap:mheap)
+  (#state:tstate)
   (#a : Type u#a)
-  (#wp1 : st_wp_h heap.t a)
-  (#wp2 : st_wp_h heap.t a)
-  (v : mst heap a wp1)
+  (#wp1 : st_wp_h state.t a)
+  (#wp2 : st_wp_h state.t a)
+  (v : mst state a wp1)
   :
-  Pure (mst heap a wp2) (requires (wp1 ⊑ wp2)) (ensures (fun _ -> True)) =
+  Pure (mst state a wp2) (requires (wp1 ⊑ wp2)) (ensures (fun _ -> True)) =
   v
 
-let partial_return heap (pre:pure_pre) : mst heap (squash pre) (partial_call_wp heap.t pre) =
+let partial_return state (pre:pure_pre) : mst state (squash pre) (partial_call_wp state.t pre) =
   PartialCall pre (Return)
 
-let get #heap () : mst heap heap.t (fun p h0 -> p h0 h0) =
+let get #state () : mst state state.t (fun p h0 -> p h0 h0) =
   Get Return
 
-let put #heap (h1:heap.t) : mst heap unit (fun p h0 -> (h0 `heap.rel` h1) /\ p () h1) =
+let put #state (h1:state.t) : mst state unit (fun p h0 -> (h0 `state.rel` h1) /\ p () h1) =
   Put h1 Return
 
-let witness #heap (pred:heap.t -> Type0) : mst heap unit (fun p h -> pred h /\ stable pred /\ (W.witnessed heap.rel pred ==> p () h)) =
+let witness #state (pred:state.t -> Type0) : mst state unit (fun p h -> pred h /\ stable pred /\ (W.witnessed state.rel pred ==> p () h)) =
   Witness pred Return
 
-let recall #heap (pred:heap.t -> Type0) : mst heap unit (fun p h -> W.witnessed heap.rel pred /\ (pred h ==> p () h)) =
+let recall #state (pred:state.t -> Type0) : mst state unit (fun p h -> W.witnessed state.rel pred /\ (pred h ==> p () h)) =
   Recall pred Return
 
-let nat_heap = {
+let nat_state = {
   t = nat;
   rel = (fun x y -> x <= y == true);
 }
 
-assume val div : #heap:mheap -> x:int -> y:int -> mst heap int (fun p h -> y <> 0 /\ p (x/y) h)
+assume val div : #state:tstate -> x:int -> y:int -> mst state int (fun p h -> y <> 0 /\ p (x/y) h)
 
 
 // put(get() + 1); witness (fun s -> s > 0); let f () = recall (fun s -> s > 0); 1 / get() in f () 0
 
-let f () : mst nat_heap int (fun p h0 -> W.witnessed nat_heap.rel (fun s -> s > 0) /\ (forall r. p r h0)) =
+let f () : mst nat_state int (fun p h0 -> W.witnessed nat_state.rel (fun s -> s > 0) /\ (forall r. p r h0)) =
   (get ())
   `mst_bind`
   (fun h -> 
@@ -124,7 +124,7 @@ let f () : mst nat_heap int (fun p h0 -> W.witnessed nat_heap.rel (fun s -> s > 
     (fun () ->
       (1 `div` h)))
 
-let test () : mst nat_heap int (fun p h0 -> forall r. p r (h0+1)) =
+let test () : mst nat_state int (fun p h0 -> forall r h1. p r h1) =
   (get ())
   `mst_bind`
   (fun h0 -> 
@@ -133,4 +133,7 @@ let test () : mst nat_heap int (fun p h0 -> forall r. p r (h0+1)) =
     (fun () -> 
       witness (fun s -> s > 0)
       `mst_bind`
-      f))
+      (fun () -> 
+        put (h0+1) // TODO: can I revert the state to h0?
+        `mst_bind`
+        (fun () -> f ()))))
