experiments/dm4ms/TOTAL_MST2.fst
@@ -1,0 +1,113 @@
+module TOTAL_MST2
+
+open WMonad
+
+
+open FStar.Tactics
+module W = FStar.Monotonic.Witnessed
+
+noeq type tstate = {
+  t: Type0;
+  rel: FStar.Preorder.preorder t;
+}
+
+let stable (#state) (pred:state.t -> Type0) =
+  forall h1 h2. (pred h1 /\ h1 `state.rel` h2) ==> pred h2
+
+type m (state:tstate) (a:Type u#a) =
+  state.t -> state.t * a
+
+let m_return (state:tstate) (a:Type) (x:a) : m state a =
+  fun h -> (h, x)
+
+let m_bind
+  (state:tstate)
+  (a:Type u#a)
+  (b:Type u#b)
+  (l : m state a)
+  (k : a -> m state b)
+  : m state b =
+  fun h0 ->
+    let (h1, v) = l h0 in
+    k v h1
+
+let partial_call_wp (state:Type0) (pre:pure_pre) : st_wp_h state (squash pre) = 
+  fun p h0 -> pre /\ p () h0
+
+val theta : #a:Type u#a -> #state:tstate -> m state a -> st_wp_h state.t a
+let rec theta #a #state m =
+  fun p h0 -> exists h1 v. h0 `state.rel` h1 /\ m h0 == (h1, v) /\ p v h1
+
+let mst (state:tstate) (a:Type) (wp:st_wp_h state.t a)=
+  mm:(m state a){theta mm ⊑ wp}
+
+let mst_return state (a:Type) (x:a) : mst state a (st_return state.t _ x) =
+  m_return state a x
+
+let mst_bind
+  (#state:tstate)
+  (#a : Type u#a)
+  (#b : Type u#b)
+  (#wp_v : st_wp_h state.t a)
+  (#wp_f: a -> st_wp_h state.t b)
+  (v : mst state a wp_v)
+  (f : (x:a -> mst state b (wp_f x))) :
+  Tot (mst state b (st_bind_wp state.t a b wp_v wp_f)) =
+  admit (); (* TODO: prove monad morphism *)
+  m_bind state a b v f
+
+let mst_subcomp
+  (#state:tstate)
+  (#a : Type u#a)
+  (#wp1 : st_wp_h state.t a)
+  (#wp2 : st_wp_h state.t a)
+  (v : mst state a wp1)
+  :
+  Pure (mst state a wp2) (requires (wp1 ⊑ wp2)) (ensures (fun _ -> True)) =
+  v
+
+// let partial_return state (pre:pure_pre) : mst state (squash pre) (partial_call_wp state.t pre) =
+//   fun h0 -> (h0, ())
+
+let get #state () : mst state state.t (fun p h0 -> p h0 h0) =
+  fun h0 -> (h0, h0)
+
+let put #state (h1:state.t) : mst state unit (fun p h0 -> (h0 `state.rel` h1) /\ p () h1) =
+  fun _ -> (h1, ())
+
+assume val witness #state (pred:state.t -> Type0) : mst state unit (fun p h -> pred h /\ stable pred /\ (W.witnessed state.rel pred ==> p () h))
+
+assume val recall #state (pred:state.t -> Type0) : mst state unit (fun p h -> W.witnessed state.rel pred /\ (pred h ==> p () h)) 
+
+let nat_state = {
+  t = nat;
+  rel = (fun x y -> x <= y == true);
+}
+
+assume val div : #state:tstate -> x:int -> y:int -> mst state int (fun p h -> y <> 0 /\ p (x/y) h)
+
+
+// put(get() + 1); witness (fun s -> s > 0); let f () = recall (fun s -> s > 0); 1 / get() in f () 0
+
+let f () : mst nat_state int (fun p h0 -> W.witnessed nat_state.rel (fun s -> s > 0) /\ (forall r. p r h0)) =
+  (get ())
+  `mst_bind`
+  (fun h -> 
+    (recall (fun s -> s > 0))
+    `mst_bind`
+    (fun () ->
+      (1 `div` h)))
+
+let test () : mst nat_state int (fun p h0 -> forall r. p r (h0+1)) =
+  (get ())
+  `mst_bind`
+  (fun h0 -> 
+    (put (h0 + 1))
+    `mst_bind`
+    (fun () -> 
+      mst_return nat_state unit () // I don't even need the witness? witness (fun s -> s > 0)
+      `mst_bind`
+      (fun () ->
+        (fun hi -> (** here I directly use the state monad *)
+          let (_, r) = f () 0 in (** I can call f with state 0 *)
+          (hi, r)) <: mst nat_state int (fun p h -> (forall r. p r h)))))
